fixed grammar errors

ironfleet/src/Dafny/Distributed/Protocol/Lock/myproof.i.dfy
@@ -10,13 +10,14 @@ import opened Types_i
 import opened DistributedSystem_i
 import opened Refinement_i
 
-predicate Service_Correspondence(concretePkts:set<LPacket<EndPoint, seq<byte>>>, serviceState:ServiceState) 
+predicate Service_Correspondence(concretePkts:set<LPacket<EndPoint, LockMessage>>, serviceState:ServiceState) 
 {
     forall p, epoch :: 
         p in concretePkts 
      && p.src in serviceState.hosts 
      && p.dst in serviceState.hosts 
-     && p.msg == MarshallLockMsg(epoch) 
+     && p.msg.Locked?
+     && p.msg.locked_epoch == epoch
      ==>
         1 <= epoch <= |serviceState.history|
      && p.src == serviceState.history[epoch-1]
@@ -40,28 +41,28 @@ lemma ForNext(gls:GLS_State, gls':GLS_State, s:ServiceState, s':ServiceState, id
     requires GLS_Next(gls, gls');
     ensures  Service_Next(s, s');
 {
-    assert gls.ls.servers == gls'.ls.servers || (gls'.ls.servers == gls.ls.servers[gls.ls.environment.nextStep.actor := s'.servers[gls.ls.environment.nextStep.actor]]);
+    assert gls.ls.servers == gls'.ls.servers || (gls'.ls.servers == gls.ls.servers[gls.ls.environment.nextStep.actor := gls'.ls.servers[gls.ls.environment.nextStep.actor]]);
     assert s'.hosts == s.hosts;
-    assert s'.history == s.history + [s.ls.servers[s.ls.environment.nextStep.actor].config[(s.ls.servers[s.ls.environment.nextStep.actor].my_index + 1) % |s.ls.servers[s.ls.environment.nextStep.actor].config|]];
+    assert s'.history == s.history + [gls.ls.servers[gls.ls.environment.nextStep.actor].config[(gls.ls.servers[gls.ls.environment.nextStep.actor].my_index + 1) % |gls.ls.servers[gls.ls.environment.nextStep.actor].config|]];
 }
 
 lemma ForCorrospondence(gls:GLS_State, gls':GLS_State, s:ServiceState, s':ServiceState)
     requires s == AbstractifyGLS_State(gls);
     requires s' == AbstractifyGLS_State(gls');
-    requires Service_Correspondence(gls.environment.sentPackets, s);
+    requires Service_Correspondence(gls.ls.environment.sentPackets, s);
     requires GLS_Next(gls, gls');
-    ensures  Service_Correspondence(gls'.environment.sentPackets, s');
+    ensures  Service_Correspondence(gls'.ls.environment.sentPackets, s');
 {
     assert if    gls.ls.environment.nextStep.LEnvStepHostIos? && gls.ls.environment.nextStep.actor in gls.ls.servers
               && NodeGrant(gls.ls.servers[gls.ls.environment.nextStep.actor], gls'.ls.servers[gls.ls.environment.nextStep.actor], gls.ls.environment.nextStep.ios)
-              && gls.ls.servers[gls.ls.environment.nextStep.actor].held && gls.ls.servers[s.ls.environment.nextStep.actor].epoch < 0xFFFF_FFFF_FFFF_FFFF then
-                     s'.history == s.history + [s.ls.servers[s.ls.environment.nextStep.actor].config[(s.ls.servers[s.ls.environment.nextStep.actor].my_index + 1) % |s.ls.servers[s.ls.environment.nextStep.actor].config|]]
-                  && gls.ls.environment.nextStep.ios.LIoOpSend?
-                  && gls'.ls.environment.sentPackets == gls.ls.environment.sentPackets + {gls.ls.environment.nextStep.ios.s}
-                  && var pkg := gls.ls.environment.nextStep.ios.s;
-                        s'.history[pkg.epoch-2] == s.ls.servers[s.ls.environment.nextStep.actor]
-                     && s.ls.servers[s.ls.environment.nextStep.actor] == pkg.src
-            else s'.history == s.history && gls.environment.sentPackets == gls'.environment.sentPackets;
+              && gls.ls.servers[gls.ls.environment.nextStep.actor].held && gls.ls.servers[gls.ls.environment.nextStep.actor].epoch < 0xFFFF_FFFF_FFFF_FFFF then
+                     s'.history == s.history + [gls.ls.servers[gls.ls.environment.nextStep.actor].config[(gls.ls.servers[gls.ls.environment.nextStep.actor].my_index + 1) % |gls.ls.servers[gls.ls.environment.nextStep.actor].config|]]
+                  && gls.ls.environment.nextStep.ios[0].LIoOpSend?
+                  && gls'.ls.environment.sentPackets == gls.ls.environment.sentPackets + {gls.ls.environment.nextStep.ios[0].s}
+                  && var pkg := gls.ls.environment.nextStep.ios[0].s;
+                        s'.history[pkg.msg.transfer_epoch-2] == gls.ls.environment.nextStep.actor
+                     && gls.ls.environment.nextStep.actor == pkg.src
+            else s'.history == s.history && gls.ls.environment.sentPackets == gls'.ls.environment.sentPackets;
 }
 
 lemma RefinementProof(config:Config, db:seq<GLS_State>) returns (sb:seq<ServiceState>)
@@ -71,23 +72,28 @@ lemma RefinementProof(config:Config, db:seq<GLS_State>) returns (sb:seq<ServiceS
     ensures  |db| == |sb|;
     ensures  Service_Init(sb[0], Collections__Maps2_s.mapdomain(db[0].ls.servers));
     ensures  forall i {:trigger Service_Next(sb[i], sb[i+1])} :: 0 <= i < |sb| - 1 ==> sb[i] == sb[i+1] || Service_Next(sb[i], sb[i+1]);
-    ensures  forall i :: 0 <= i < |db| ==> Service_Correspondence(db[i].environment.sentPackets, sb[i]);
+    ensures  forall i :: 0 <= i < |db| ==> Service_Correspondence(db[i].ls.environment.sentPackets, sb[i]);
 {
     sb:=[AbstractifyGLS_State(db[0])];
     ForInit(db[0], sb[0], config);
 
     var i := 1;
     while (i < |db|)
-      invariant  Service_Init(sb[0], Collections__Maps2_s.mapdomain(db[0].servers));
+      invariant  Service_Init(sb[0], Collections__Maps2_s.mapdomain(db[0].ls.servers));
       invariant  forall i {:trigger Service_Next(sb[i], sb[i+1])} :: 0 <= i < |sb| - 1 ==> sb[i] == sb[i+1] || Service_Next(sb[i], sb[i+1]);
-      invariant  forall i :: 0 <= i < |sb| ==> Service_Correspondence(db[i].environment.sentPackets, sb[i]);
+      invariant  forall i :: 0 <= i < |sb| ==> Service_Correspondence(db[i].ls.environment.sentPackets, sb[i]);
       invariant  |sb| == i;
     {
         sb := sb + [AbstractifyGLS_State(db[i])];
         
-        assert if db[i-1].environment.nextStep.LEnvStepHostIos? && db[i-1].environment.nextStep.actor in s.servers then
-                    ForNext(db[i-1], db[i], sb[i-1], sb[i], db[i-1].environment.nextStep.actor)
-                else sb[i-1] == sb[i];
+        if db[i-1].ls.environment.nextStep.LEnvStepHostIos? && db[i-1].ls.environment.nextStep.actor in config
+        {
+            ForNext(db[i-1], db[i], sb[i-1], sb[i], db[i-1].ls.environment.nextStep.actor);
+        }
+        else
+        {
+            assert sb[i-1] == sb[i];
+        }
         ForCorrospondence(db[i-1], db[i], sb[i-1], sb[i]);
 
         i := i+1;
